clean up array_swap, with an interface

pulse/share/steel/examples/pulse/lib/Pulse.Lib.ArraySwap.fst
@@ -1,13 +1,10 @@
 module Pulse.Lib.ArraySwap
-open Pulse.Lib.Pervasives
-module U32 = FStar.UInt32
-module Prf = Steel.ST.GenArraySwap.Proof
-module SZ = FStar.SizeT
-module A = Pulse.Lib.Array
 module R = Pulse.Lib.Reference
+module Prf = Steel.ST.GenArraySwap.Proof
 #push-options "--using_facts_from '* -FStar.Tactics -FStar.Reflection' --fuel 2 --ifuel 1"
 #restart-solver
 
+inline_for_extraction
 ```pulse
 fn gcd (n0: SZ.t) (l0: SZ.t)
   requires (emp ** pure (
@@ -88,73 +85,16 @@ let size_sub
 : Tot (c: SZ.t { SZ.v c == (SZ.v a - SZ.v b) })
 = a `SZ.sub` b
 
-(*
-```pulse
-fn get_array_pts_to (#t: Type0) (#p: perm) (#s: Ghost.erased (Seq.seq t)) (a: A.array t)
-  requires (A.pts_to a p s)
-  returns s': Ghost.erased (Seq.seq t)
-  ensures (A.pts_to a p s ** pure (s' == s))
-  {
-    s
-  }
-```
-*)
-
-(*
-assume val get_array_pts_to (#opened: _) (#t: Type0) (#p: perm) (#s: Seq.seq t) (a: A.array t)
-: stt_ghost (Ghost.erased (Seq.seq t)) opened
-    (A.pts_to a p s)
-    (fun s' -> A.pts_to a p s ** pure (Ghost.reveal s' == s))
-*)
-
-(*
-assume val get_array_pts_to (#t: Type0) (#p: perm) (#s: Ghost.erased (Seq.seq t)) (a: A.array t)
-: stt (Ghost.erased (Seq.seq t))
-    (A.pts_to a p s)
-    (fun s' -> A.pts_to a p s ** pure (s' == s))
-*)
-
-```pulse
-fn get_array_pts_to (#t: Type0) (a: A.array t) (#p: perm) (#s: Ghost.erased (Seq.seq t))
-  requires A.pts_to a #p s
-  returns s': Ghost.erased (Seq.seq t)
-  ensures A.pts_to a #p s ** pure (s' == s)
-  {
-    s
-  }
-```
-
-```pulse
-fn get_pts_to (#t: Type0) (a: ref t) (#p: perm) (#s: erased (t))
-  requires pts_to a #p s
-  returns s': Ghost.erased (t)
-  ensures pts_to a #p s ** pure (s' == s)
-  {
-    s
-  }
-```
-
-```pulse
-fn pulse_assert (p: prop)
-  requires (pure p)
-  returns res: squash p
-  ensures emp
-  {
-    ()
-  }
-```
-
 #restart-solver
 
 #push-options "--z3rlimit_factor 4"
 
 inline_for_extraction noextract [@@noextract_to "krml"]
 ```pulse
-fn array_swap'(#t: Type0) (#s0: Ghost.erased (Seq.seq t)) (a: A.array t) (lb: SZ.t) (rb: SZ.t) (mb: (mb: SZ.t {SZ.v mb > SZ.v lb /\ SZ.v mb < SZ.v rb})) (bz: Prf.bezout (SZ.v rb - SZ.v lb) (SZ.v mb - SZ.v lb)) (d: SZ.t) (q: SZ.t)
+fn array_swap_aux(#t: Type0) (a: A.array t) (lb: SZ.t) (rb: SZ.t) (mb: (mb: SZ.t {SZ.v mb > SZ.v lb /\ SZ.v mb < SZ.v rb})) (bz: Prf.bezout (SZ.v rb - SZ.v lb) (SZ.v mb - SZ.v lb)) (d: SZ.t) (q: SZ.t) (#s0: Ghost.erased (Seq.seq t))
   requires (
     A.pts_to_range a (Ghost.reveal (SZ.v lb)) (Ghost.reveal (SZ.v rb)) s0 **
     pure (
-      Seq.length s0 == SZ.v rb - SZ.v lb /\
       SZ.v d == bz.d /\
       SZ.v q == bz.q_n
     )
@@ -164,6 +104,7 @@ fn array_swap'(#t: Type0) (#s0: Ghost.erased (Seq.seq t)) (a: A.array t) (lb: SZ
     pure (Prf.array_swap_post s0 (SZ.v rb - SZ.v lb) (SZ.v mb - SZ.v lb) s) // hoisted out because of the SMT pattern on array_as_ring_buffer_swap
   )
 {   
+    A.pts_to_range_prop a;
     let mut pi = lb;
     while (let i = !pi; ((i `SZ.sub` lb) `size_lt` d))
     invariant b . exists s i . (
@@ -212,3 +153,102 @@ fn array_swap'(#t: Type0) (#s0: Ghost.erased (Seq.seq t)) (a: A.array t) (lb: SZ
     ()
 }
 ```
+
+#pop-options
+
+let seq_slice_full
+  (#t: Type)
+  (s: Seq.seq t)
+: Lemma
+  (s == Seq.slice s 0 (Seq.length s))
+= assert (s `Seq.equal` Seq.slice s 0 (Seq.length s))
+
+```pulse
+ghost
+fn manurewrite
+  (p: vprop)
+  (q: vprop)
+requires p ** pure (p == q)
+ensures q
+{
+  rewrite p as q
+}
+```
+
+inline_for_extraction noextract [@@noextract_to "krml"]
+```pulse
+fn array_swap0
+  (#t: Type0)
+  (a: A.array t)
+  (lb: SZ.t) (rb: SZ.t)
+  (mb: SZ.t)
+  (#s1 #s2: Ghost.erased (Seq.seq t))
+requires (
+    A.pts_to_range a (SZ.v lb) (SZ.v mb) s1 **
+    A.pts_to_range a (SZ.v mb) (SZ.v rb) s2
+  )
+returns prf: squash (SZ.v lb <= SZ.v mb /\ SZ.v mb <= SZ.v rb)
+ensures (
+    A.pts_to_range a (SZ.v lb) (SZ.v lb + (SZ.v rb - SZ.v mb)) s2 **
+    A.pts_to_range a (SZ.v lb + (SZ.v rb - SZ.v mb)) (SZ.v rb) s1
+  )
+{
+  A.pts_to_range_prop a #(SZ.v lb) #(SZ.v mb);
+  A.pts_to_range_prop a #(SZ.v mb) #(SZ.v rb);
+  let prf : squash (SZ.v lb <= SZ.v mb /\ SZ.v mb <= SZ.v rb) = ();
+  A.pts_to_range_join a (SZ.v lb) (SZ.v mb) (SZ.v rb);
+  with s . assert (A.pts_to_range a (SZ.v lb) (SZ.v rb) s);
+  if (lb = mb) {
+    let prf_s1 : squash (s1 `Seq.equal` Seq.empty) = ();
+    let prf_s : squash (s2 `Seq.equal` s) = ();
+    A.pts_to_range_split a (SZ.v lb) (SZ.v rb) (SZ.v rb);
+    with s2' . assert (A.pts_to_range a (SZ.v lb) (SZ.v rb) s2');
+    with s1' . assert (A.pts_to_range a (SZ.v rb) (SZ.v rb) s1');
+    let prf1 : squash (s1' `Seq.equal` s1) = ();
+    let prf2 : squash (s2' `Seq.equal` s2) = ();
+    let prf_mb : squash (SZ.v mb == SZ.v lb /\ SZ.v lb + (SZ.v rb - SZ.v mb) == SZ.v rb) = ();
+    rewrite (A.pts_to_range a (SZ.v lb) (SZ.v rb) s2')
+      as (A.pts_to_range a (SZ.v lb) (SZ.v lb + (SZ.v rb - SZ.v mb)) s2);
+    rewrite (A.pts_to_range a (SZ.v rb) (SZ.v rb) s1')
+      as (A.pts_to_range a (SZ.v lb + (SZ.v rb - SZ.v mb)) (SZ.v rb) s1);
+    prf
+  } else if (mb = rb) {
+    let prf_s2 : squash (s2 `Seq.equal` Seq.empty) = ();
+    let prf_s : squash (s1 `Seq.equal` s) = ();
+    A.pts_to_range_split a (SZ.v lb) (SZ.v lb) (SZ.v rb);
+    with s2' . assert (A.pts_to_range a (SZ.v lb) (SZ.v lb) s2');
+    with s1' . assert (A.pts_to_range a (SZ.v lb) (SZ.v rb) s1');
+    let prf1 : squash (s1' `Seq.equal` s1) = ();
+    let prf2 : squash (s2' `Seq.equal` s2) = ();
+    let prf_mb : squash (SZ.v mb == SZ.v rb /\ SZ.v lb + (SZ.v rb - SZ.v mb) == SZ.v lb) = ();
+    rewrite (A.pts_to_range a (SZ.v lb) (SZ.v lb) s2')
+      as (A.pts_to_range a (SZ.v lb) (SZ.v lb + (SZ.v rb - SZ.v mb)) s2);
+    rewrite (A.pts_to_range a (SZ.v lb) (SZ.v rb) s1')
+      as (A.pts_to_range a (SZ.v lb + (SZ.v rb - SZ.v mb)) (SZ.v rb) s1);
+    prf
+  } else {
+    Seq.lemma_split s (SZ.v mb - SZ.v lb);
+    Seq.lemma_append_inj s1 s2 (Seq.slice s 0 (SZ.v mb - SZ.v lb)) (Seq.slice s (SZ.v mb - SZ.v lb) (Seq.length s));
+    rewrite (A.pts_to_range a (SZ.v lb) (SZ.v rb) s)
+      as (A.pts_to_range a (Ghost.reveal (SZ.v lb)) (Ghost.reveal (SZ.v rb)) s);
+    let d = gcd (rb `SZ.sub` lb) (mb `SZ.sub` lb);
+    let q = (rb `SZ.sub` lb) `SZ.div` d;
+    array_swap_aux a lb rb mb (Prf.mk_bezout _ _) d q;
+    with s' . assert (A.pts_to_range a (Ghost.reveal (SZ.v lb)) (Ghost.reveal (SZ.v rb)) s');
+    rewrite (A.pts_to_range a (Ghost.reveal (SZ.v lb)) (Ghost.reveal (SZ.v rb)) s')
+      as (A.pts_to_range a (SZ.v lb) (SZ.v rb) s');
+    Seq.lemma_split s' (SZ.v rb - SZ.v mb);
+    Seq.lemma_append_inj s2 s1 (Seq.slice s' 0 (SZ.v rb - SZ.v mb)) (Seq.slice s' (SZ.v rb - SZ.v mb) (Seq.length s'));
+    A.pts_to_range_split a (SZ.v lb) (SZ.v lb + (SZ.v rb - SZ.v mb)) (SZ.v rb);
+    with s2' . assert (A.pts_to_range a (SZ.v lb) (SZ.v lb + (SZ.v rb - SZ.v mb)) s2');
+    rewrite (A.pts_to_range a (SZ.v lb) (SZ.v lb + (SZ.v rb - SZ.v mb)) s2')
+      as (A.pts_to_range a (SZ.v lb) (SZ.v lb + (SZ.v rb - SZ.v mb)) s2);
+    with s1' . assert (A.pts_to_range a (SZ.v lb + (SZ.v rb - SZ.v mb)) (SZ.v rb) s1');
+    rewrite (A.pts_to_range a (SZ.v lb + (SZ.v rb - SZ.v mb)) (SZ.v rb) s1')
+      as (A.pts_to_range a (SZ.v lb + (SZ.v rb - SZ.v mb)) (SZ.v rb) s1);
+    prf
+  }
+}
+```
+
+let array_swap = array_swap0
