pulse/share/steel/examples/pulse/lib/Pulse.Lib.ArraySwap.fsti
@@ -1,0 +1,21 @@
+module Pulse.Lib.ArraySwap
+open Pulse.Lib.Pervasives
+module SZ = FStar.SizeT
+module A = Pulse.Lib.Array
+
+inline_for_extraction noextract [@@noextract_to "krml"]
+val array_swap
+  (#t: Type0)
+  (a: A.array t)
+  (lb: SZ.t) (rb: SZ.t)
+  (mb: SZ.t)
+  (#s1 #s2: Ghost.erased (Seq.seq t))
+: stt (squash (SZ.v lb <= SZ.v mb /\ SZ.v mb <= SZ.v rb))
+  (
+    A.pts_to_range a (SZ.v lb) (SZ.v mb) s1 **
+    A.pts_to_range a (SZ.v mb) (SZ.v rb) s2
+  )
+  (fun _ ->
+    A.pts_to_range a (SZ.v lb) (SZ.v lb + (SZ.v rb - SZ.v mb)) s2 **
+    A.pts_to_range a (SZ.v lb + (SZ.v rb - SZ.v mb)) (SZ.v rb) s1
+  )
